Seems to work but takes a million years to type check

theories/Autosubst2/syntax.v
@@ -1,4 +1,4 @@
-Require Import core fintype.
+Require Import core unscoped.
 
 Require Import Setoid Morphisms Relation_Definitions.
 
@@ -33,221 +33,177 @@ Proof.
 exact (eq_refl).
 Qed.
 
-Inductive PTm (n_PTm : nat) : Type :=
-  | VarPTm : fin n_PTm -> PTm n_PTm
-  | PAbs : PTm (S n_PTm) -> PTm n_PTm
-  | PApp : PTm n_PTm -> PTm n_PTm -> PTm n_PTm
-  | PPair : PTm n_PTm -> PTm n_PTm -> PTm n_PTm
-  | PProj : PTag -> PTm n_PTm -> PTm n_PTm
-  | PBind : BTag -> PTm n_PTm -> PTm (S n_PTm) -> PTm n_PTm
-  | PUniv : nat -> PTm n_PTm
-  | PBot : PTm n_PTm
-  | PNat : PTm n_PTm
-  | PZero : PTm n_PTm
-  | PSuc : PTm n_PTm -> PTm n_PTm
-  | PInd :
-      PTm (S n_PTm) ->
-      PTm n_PTm -> PTm n_PTm -> PTm (S (S n_PTm)) -> PTm n_PTm.
+Inductive PTm : Type :=
+  | VarPTm : nat -> PTm
+  | PAbs : PTm -> PTm
+  | PApp : PTm -> PTm -> PTm
+  | PPair : PTm -> PTm -> PTm
+  | PProj : PTag -> PTm -> PTm
+  | PBind : BTag -> PTm -> PTm -> PTm
+  | PUniv : nat -> PTm
+  | PBot : PTm
+  | PNat : PTm
+  | PZero : PTm
+  | PSuc : PTm -> PTm
+  | PInd : PTm -> PTm -> PTm -> PTm -> PTm.
 
-Lemma congr_PAbs {m_PTm : nat} {s0 : PTm (S m_PTm)} {t0 : PTm (S m_PTm)}
-  (H0 : s0 = t0) : PAbs m_PTm s0 = PAbs m_PTm t0.
+Lemma congr_PAbs {s0 : PTm} {t0 : PTm} (H0 : s0 = t0) : PAbs s0 = PAbs t0.
 Proof.
-exact (eq_trans eq_refl (ap (fun x => PAbs m_PTm x) H0)).
+exact (eq_trans eq_refl (ap (fun x => PAbs x) H0)).
 Qed.
 
-Lemma congr_PApp {m_PTm : nat} {s0 : PTm m_PTm} {s1 : PTm m_PTm}
-  {t0 : PTm m_PTm} {t1 : PTm m_PTm} (H0 : s0 = t0) (H1 : s1 = t1) :
-  PApp m_PTm s0 s1 = PApp m_PTm t0 t1.
+Lemma congr_PApp {s0 : PTm} {s1 : PTm} {t0 : PTm} {t1 : PTm} (H0 : s0 = t0)
+  (H1 : s1 = t1) : PApp s0 s1 = PApp t0 t1.
 Proof.
-exact (eq_trans (eq_trans eq_refl (ap (fun x => PApp m_PTm x s1) H0))
-         (ap (fun x => PApp m_PTm t0 x) H1)).
+exact (eq_trans (eq_trans eq_refl (ap (fun x => PApp x s1) H0))
+         (ap (fun x => PApp t0 x) H1)).
 Qed.
 
-Lemma congr_PPair {m_PTm : nat} {s0 : PTm m_PTm} {s1 : PTm m_PTm}
-  {t0 : PTm m_PTm} {t1 : PTm m_PTm} (H0 : s0 = t0) (H1 : s1 = t1) :
-  PPair m_PTm s0 s1 = PPair m_PTm t0 t1.
+Lemma congr_PPair {s0 : PTm} {s1 : PTm} {t0 : PTm} {t1 : PTm} (H0 : s0 = t0)
+  (H1 : s1 = t1) : PPair s0 s1 = PPair t0 t1.
 Proof.
-exact (eq_trans (eq_trans eq_refl (ap (fun x => PPair m_PTm x s1) H0))
-         (ap (fun x => PPair m_PTm t0 x) H1)).
+exact (eq_trans (eq_trans eq_refl (ap (fun x => PPair x s1) H0))
+         (ap (fun x => PPair t0 x) H1)).
 Qed.
 
-Lemma congr_PProj {m_PTm : nat} {s0 : PTag} {s1 : PTm m_PTm} {t0 : PTag}
-  {t1 : PTm m_PTm} (H0 : s0 = t0) (H1 : s1 = t1) :
-  PProj m_PTm s0 s1 = PProj m_PTm t0 t1.
+Lemma congr_PProj {s0 : PTag} {s1 : PTm} {t0 : PTag} {t1 : PTm}
+  (H0 : s0 = t0) (H1 : s1 = t1) : PProj s0 s1 = PProj t0 t1.
 Proof.
-exact (eq_trans (eq_trans eq_refl (ap (fun x => PProj m_PTm x s1) H0))
-         (ap (fun x => PProj m_PTm t0 x) H1)).
+exact (eq_trans (eq_trans eq_refl (ap (fun x => PProj x s1) H0))
+         (ap (fun x => PProj t0 x) H1)).
 Qed.
 
-Lemma congr_PBind {m_PTm : nat} {s0 : BTag} {s1 : PTm m_PTm}
-  {s2 : PTm (S m_PTm)} {t0 : BTag} {t1 : PTm m_PTm} {t2 : PTm (S m_PTm)}
-  (H0 : s0 = t0) (H1 : s1 = t1) (H2 : s2 = t2) :
-  PBind m_PTm s0 s1 s2 = PBind m_PTm t0 t1 t2.
+Lemma congr_PBind {s0 : BTag} {s1 : PTm} {s2 : PTm} {t0 : BTag} {t1 : PTm}
+  {t2 : PTm} (H0 : s0 = t0) (H1 : s1 = t1) (H2 : s2 = t2) :
+  PBind s0 s1 s2 = PBind t0 t1 t2.
 Proof.
 exact (eq_trans
-         (eq_trans (eq_trans eq_refl (ap (fun x => PBind m_PTm x s1 s2) H0))
-            (ap (fun x => PBind m_PTm t0 x s2) H1))
-         (ap (fun x => PBind m_PTm t0 t1 x) H2)).
+         (eq_trans (eq_trans eq_refl (ap (fun x => PBind x s1 s2) H0))
+            (ap (fun x => PBind t0 x s2) H1))
+         (ap (fun x => PBind t0 t1 x) H2)).
 Qed.
 
-Lemma congr_PUniv {m_PTm : nat} {s0 : nat} {t0 : nat} (H0 : s0 = t0) :
-  PUniv m_PTm s0 = PUniv m_PTm t0.
+Lemma congr_PUniv {s0 : nat} {t0 : nat} (H0 : s0 = t0) : PUniv s0 = PUniv t0.
 Proof.
-exact (eq_trans eq_refl (ap (fun x => PUniv m_PTm x) H0)).
+exact (eq_trans eq_refl (ap (fun x => PUniv x) H0)).
 Qed.
 
-Lemma congr_PBot {m_PTm : nat} : PBot m_PTm = PBot m_PTm.
-Proof.
-exact (eq_refl).
-Qed.
-
-Lemma congr_PNat {m_PTm : nat} : PNat m_PTm = PNat m_PTm.
+Lemma congr_PBot : PBot = PBot.
 Proof.
 exact (eq_refl).
 Qed.
 
-Lemma congr_PZero {m_PTm : nat} : PZero m_PTm = PZero m_PTm.
+Lemma congr_PNat : PNat = PNat.
 Proof.
 exact (eq_refl).
 Qed.
 
-Lemma congr_PSuc {m_PTm : nat} {s0 : PTm m_PTm} {t0 : PTm m_PTm}
-  (H0 : s0 = t0) : PSuc m_PTm s0 = PSuc m_PTm t0.
+Lemma congr_PZero : PZero = PZero.
 Proof.
-exact (eq_trans eq_refl (ap (fun x => PSuc m_PTm x) H0)).
+exact (eq_refl).
 Qed.
 
-Lemma congr_PInd {m_PTm : nat} {s0 : PTm (S m_PTm)} {s1 : PTm m_PTm}
-  {s2 : PTm m_PTm} {s3 : PTm (S (S m_PTm))} {t0 : PTm (S m_PTm)}
-  {t1 : PTm m_PTm} {t2 : PTm m_PTm} {t3 : PTm (S (S m_PTm))} (H0 : s0 = t0)
-  (H1 : s1 = t1) (H2 : s2 = t2) (H3 : s3 = t3) :
-  PInd m_PTm s0 s1 s2 s3 = PInd m_PTm t0 t1 t2 t3.
+Lemma congr_PSuc {s0 : PTm} {t0 : PTm} (H0 : s0 = t0) : PSuc s0 = PSuc t0.
+Proof.
+exact (eq_trans eq_refl (ap (fun x => PSuc x) H0)).
+Qed.
+
+Lemma congr_PInd {s0 : PTm} {s1 : PTm} {s2 : PTm} {s3 : PTm} {t0 : PTm}
+  {t1 : PTm} {t2 : PTm} {t3 : PTm} (H0 : s0 = t0) (H1 : s1 = t1)
+  (H2 : s2 = t2) (H3 : s3 = t3) : PInd s0 s1 s2 s3 = PInd t0 t1 t2 t3.
 Proof.
 exact (eq_trans
          (eq_trans
-            (eq_trans
-               (eq_trans eq_refl (ap (fun x => PInd m_PTm x s1 s2 s3) H0))
-               (ap (fun x => PInd m_PTm t0 x s2 s3) H1))
-            (ap (fun x => PInd m_PTm t0 t1 x s3) H2))
-         (ap (fun x => PInd m_PTm t0 t1 t2 x) H3)).
+            (eq_trans (eq_trans eq_refl (ap (fun x => PInd x s1 s2 s3) H0))
+               (ap (fun x => PInd t0 x s2 s3) H1))
+            (ap (fun x => PInd t0 t1 x s3) H2))
+         (ap (fun x => PInd t0 t1 t2 x) H3)).
 Qed.
 
-Lemma upRen_PTm_PTm {m : nat} {n : nat} (xi : fin m -> fin n) :
-  fin (S m) -> fin (S n).
+Lemma upRen_PTm_PTm (xi : nat -> nat) : nat -> nat.
 Proof.
 exact (up_ren xi).
 Defined.
 
-Lemma upRen_list_PTm_PTm (p : nat) {m : nat} {n : nat} (xi : fin m -> fin n)
-  : fin (plus p m) -> fin (plus p n).
-Proof.
-exact (upRen_p p xi).
-Defined.
-
-Fixpoint ren_PTm {m_PTm : nat} {n_PTm : nat}
-(xi_PTm : fin m_PTm -> fin n_PTm) (s : PTm m_PTm) {struct s} : PTm n_PTm :=
+Fixpoint ren_PTm (xi_PTm : nat -> nat) (s : PTm) {struct s} : PTm :=
   match s with
-  | VarPTm _ s0 => VarPTm n_PTm (xi_PTm s0)
-  | PAbs _ s0 => PAbs n_PTm (ren_PTm (upRen_PTm_PTm xi_PTm) s0)
-  | PApp _ s0 s1 => PApp n_PTm (ren_PTm xi_PTm s0) (ren_PTm xi_PTm s1)
-  | PPair _ s0 s1 => PPair n_PTm (ren_PTm xi_PTm s0) (ren_PTm xi_PTm s1)
-  | PProj _ s0 s1 => PProj n_PTm s0 (ren_PTm xi_PTm s1)
-  | PBind _ s0 s1 s2 =>
-      PBind n_PTm s0 (ren_PTm xi_PTm s1) (ren_PTm (upRen_PTm_PTm xi_PTm) s2)
-  | PUniv _ s0 => PUniv n_PTm s0
-  | PBot _ => PBot n_PTm
-  | PNat _ => PNat n_PTm
-  | PZero _ => PZero n_PTm
-  | PSuc _ s0 => PSuc n_PTm (ren_PTm xi_PTm s0)
-  | PInd _ s0 s1 s2 s3 =>
-      PInd n_PTm (ren_PTm (upRen_PTm_PTm xi_PTm) s0) (ren_PTm xi_PTm s1)
+  | VarPTm s0 => VarPTm (xi_PTm s0)
+  | PAbs s0 => PAbs (ren_PTm (upRen_PTm_PTm xi_PTm) s0)
+  | PApp s0 s1 => PApp (ren_PTm xi_PTm s0) (ren_PTm xi_PTm s1)
+  | PPair s0 s1 => PPair (ren_PTm xi_PTm s0) (ren_PTm xi_PTm s1)
+  | PProj s0 s1 => PProj s0 (ren_PTm xi_PTm s1)
+  | PBind s0 s1 s2 =>
+      PBind s0 (ren_PTm xi_PTm s1) (ren_PTm (upRen_PTm_PTm xi_PTm) s2)
+  | PUniv s0 => PUniv s0
+  | PBot => PBot
+  | PNat => PNat
+  | PZero => PZero
+  | PSuc s0 => PSuc (ren_PTm xi_PTm s0)
+  | PInd s0 s1 s2 s3 =>
+      PInd (ren_PTm (upRen_PTm_PTm xi_PTm) s0) (ren_PTm xi_PTm s1)
         (ren_PTm xi_PTm s2)
         (ren_PTm (upRen_PTm_PTm (upRen_PTm_PTm xi_PTm)) s3)
   end.
 
-Lemma up_PTm_PTm {m : nat} {n_PTm : nat} (sigma : fin m -> PTm n_PTm) :
-  fin (S m) -> PTm (S n_PTm).
+Lemma up_PTm_PTm (sigma : nat -> PTm) : nat -> PTm.
 Proof.
-exact (scons (VarPTm (S n_PTm) var_zero) (funcomp (ren_PTm shift) sigma)).
+exact (scons (VarPTm var_zero) (funcomp (ren_PTm shift) sigma)).
 Defined.
 
-Lemma up_list_PTm_PTm (p : nat) {m : nat} {n_PTm : nat}
-  (sigma : fin m -> PTm n_PTm) : fin (plus p m) -> PTm (plus p n_PTm).
-Proof.
-exact (scons_p p (funcomp (VarPTm (plus p n_PTm)) (zero_p p))
-         (funcomp (ren_PTm (shift_p p)) sigma)).
-Defined.
-
-Fixpoint subst_PTm {m_PTm : nat} {n_PTm : nat}
-(sigma_PTm : fin m_PTm -> PTm n_PTm) (s : PTm m_PTm) {struct s} : PTm n_PTm
-:=
+Fixpoint subst_PTm (sigma_PTm : nat -> PTm) (s : PTm) {struct s} : PTm :=
   match s with
-  | VarPTm _ s0 => sigma_PTm s0
-  | PAbs _ s0 => PAbs n_PTm (subst_PTm (up_PTm_PTm sigma_PTm) s0)
-  | PApp _ s0 s1 =>
-      PApp n_PTm (subst_PTm sigma_PTm s0) (subst_PTm sigma_PTm s1)
-  | PPair _ s0 s1 =>
-      PPair n_PTm (subst_PTm sigma_PTm s0) (subst_PTm sigma_PTm s1)
-  | PProj _ s0 s1 => PProj n_PTm s0 (subst_PTm sigma_PTm s1)
-  | PBind _ s0 s1 s2 =>
-      PBind n_PTm s0 (subst_PTm sigma_PTm s1)
-        (subst_PTm (up_PTm_PTm sigma_PTm) s2)
-  | PUniv _ s0 => PUniv n_PTm s0
-  | PBot _ => PBot n_PTm
-  | PNat _ => PNat n_PTm
-  | PZero _ => PZero n_PTm
-  | PSuc _ s0 => PSuc n_PTm (subst_PTm sigma_PTm s0)
-  | PInd _ s0 s1 s2 s3 =>
-      PInd n_PTm (subst_PTm (up_PTm_PTm sigma_PTm) s0)
-        (subst_PTm sigma_PTm s1) (subst_PTm sigma_PTm s2)
+  | VarPTm s0 => sigma_PTm s0
+  | PAbs s0 => PAbs (subst_PTm (up_PTm_PTm sigma_PTm) s0)
+  | PApp s0 s1 => PApp (subst_PTm sigma_PTm s0) (subst_PTm sigma_PTm s1)
+  | PPair s0 s1 => PPair (subst_PTm sigma_PTm s0) (subst_PTm sigma_PTm s1)
+  | PProj s0 s1 => PProj s0 (subst_PTm sigma_PTm s1)
+  | PBind s0 s1 s2 =>
+      PBind s0 (subst_PTm sigma_PTm s1) (subst_PTm (up_PTm_PTm sigma_PTm) s2)
+  | PUniv s0 => PUniv s0
+  | PBot => PBot
+  | PNat => PNat
+  | PZero => PZero
+  | PSuc s0 => PSuc (subst_PTm sigma_PTm s0)
+  | PInd s0 s1 s2 s3 =>
+      PInd (subst_PTm (up_PTm_PTm sigma_PTm) s0) (subst_PTm sigma_PTm s1)
+        (subst_PTm sigma_PTm s2)
         (subst_PTm (up_PTm_PTm (up_PTm_PTm sigma_PTm)) s3)
   end.
 
-Lemma upId_PTm_PTm {m_PTm : nat} (sigma : fin m_PTm -> PTm m_PTm)
-  (Eq : forall x, sigma x = VarPTm m_PTm x) :
-  forall x, up_PTm_PTm sigma x = VarPTm (S m_PTm) x.
+Lemma upId_PTm_PTm (sigma : nat -> PTm) (Eq : forall x, sigma x = VarPTm x) :
+  forall x, up_PTm_PTm sigma x = VarPTm x.
 Proof.
 exact (fun n =>
        match n with
-       | Some fin_n => ap (ren_PTm shift) (Eq fin_n)
-       | None => eq_refl
+       | S n' => ap (ren_PTm shift) (Eq n')
+       | O => eq_refl
        end).
 Qed.
 
-Lemma upId_list_PTm_PTm {p : nat} {m_PTm : nat}
-  (sigma : fin m_PTm -> PTm m_PTm) (Eq : forall x, sigma x = VarPTm m_PTm x)
-  : forall x, up_list_PTm_PTm p sigma x = VarPTm (plus p m_PTm) x.
-Proof.
-exact (fun n =>
-       scons_p_eta (VarPTm (plus p m_PTm))
-         (fun n => ap (ren_PTm (shift_p p)) (Eq n)) (fun n => eq_refl)).
-Qed.
-
-Fixpoint idSubst_PTm {m_PTm : nat} (sigma_PTm : fin m_PTm -> PTm m_PTm)
-(Eq_PTm : forall x, sigma_PTm x = VarPTm m_PTm x) (s : PTm m_PTm) {struct s}
-   : subst_PTm sigma_PTm s = s :=
+Fixpoint idSubst_PTm (sigma_PTm : nat -> PTm)
+(Eq_PTm : forall x, sigma_PTm x = VarPTm x) (s : PTm) {struct s} :
+subst_PTm sigma_PTm s = s :=
   match s with
-  | VarPTm _ s0 => Eq_PTm s0
-  | PAbs _ s0 =>
+  | VarPTm s0 => Eq_PTm s0
+  | PAbs s0 =>
       congr_PAbs
         (idSubst_PTm (up_PTm_PTm sigma_PTm) (upId_PTm_PTm _ Eq_PTm) s0)
-  | PApp _ s0 s1 =>
+  | PApp s0 s1 =>
       congr_PApp (idSubst_PTm sigma_PTm Eq_PTm s0)
         (idSubst_PTm sigma_PTm Eq_PTm s1)
-  | PPair _ s0 s1 =>
+  | PPair s0 s1 =>
       congr_PPair (idSubst_PTm sigma_PTm Eq_PTm s0)
         (idSubst_PTm sigma_PTm Eq_PTm s1)
-  | PProj _ s0 s1 =>
-      congr_PProj (eq_refl s0) (idSubst_PTm sigma_PTm Eq_PTm s1)
-  | PBind _ s0 s1 s2 =>
+  | PProj s0 s1 => congr_PProj (eq_refl s0) (idSubst_PTm sigma_PTm Eq_PTm s1)
+  | PBind s0 s1 s2 =>
       congr_PBind (eq_refl s0) (idSubst_PTm sigma_PTm Eq_PTm s1)
         (idSubst_PTm (up_PTm_PTm sigma_PTm) (upId_PTm_PTm _ Eq_PTm) s2)
-  | PUniv _ s0 => congr_PUniv (eq_refl s0)
-  | PBot _ => congr_PBot
-  | PNat _ => congr_PNat
-  | PZero _ => congr_PZero
-  | PSuc _ s0 => congr_PSuc (idSubst_PTm sigma_PTm Eq_PTm s0)
-  | PInd _ s0 s1 s2 s3 =>
+  | PUniv s0 => congr_PUniv (eq_refl s0)
+  | PBot => congr_PBot
+  | PNat => congr_PNat
+  | PZero => congr_PZero
+  | PSuc s0 => congr_PSuc (idSubst_PTm sigma_PTm Eq_PTm s0)
+  | PInd s0 s1 s2 s3 =>
       congr_PInd
         (idSubst_PTm (up_PTm_PTm sigma_PTm) (upId_PTm_PTm _ Eq_PTm) s0)
         (idSubst_PTm sigma_PTm Eq_PTm s1) (idSubst_PTm sigma_PTm Eq_PTm s2)
@@ -255,54 +211,43 @@ Fixpoint idSubst_PTm {m_PTm : nat} (sigma_PTm : fin m_PTm -> PTm m_PTm)
            (upId_PTm_PTm _ (upId_PTm_PTm _ Eq_PTm)) s3)
   end.
 
-Lemma upExtRen_PTm_PTm {m : nat} {n : nat} (xi : fin m -> fin n)
-  (zeta : fin m -> fin n) (Eq : forall x, xi x = zeta x) :
+Lemma upExtRen_PTm_PTm (xi : nat -> nat) (zeta : nat -> nat)
+  (Eq : forall x, xi x = zeta x) :
   forall x, upRen_PTm_PTm xi x = upRen_PTm_PTm zeta x.
 Proof.
-exact (fun n =>
-       match n with
-       | Some fin_n => ap shift (Eq fin_n)
-       | None => eq_refl
-       end).
+exact (fun n => match n with
+                | S n' => ap shift (Eq n')
+                | O => eq_refl
+                end).
 Qed.
 
-Lemma upExtRen_list_PTm_PTm {p : nat} {m : nat} {n : nat}
-  (xi : fin m -> fin n) (zeta : fin m -> fin n)
-  (Eq : forall x, xi x = zeta x) :
-  forall x, upRen_list_PTm_PTm p xi x = upRen_list_PTm_PTm p zeta x.
-Proof.
-exact (fun n =>
-       scons_p_congr (fun n => eq_refl) (fun n => ap (shift_p p) (Eq n))).
-Qed.
-
-Fixpoint extRen_PTm {m_PTm : nat} {n_PTm : nat}
-(xi_PTm : fin m_PTm -> fin n_PTm) (zeta_PTm : fin m_PTm -> fin n_PTm)
-(Eq_PTm : forall x, xi_PTm x = zeta_PTm x) (s : PTm m_PTm) {struct s} :
+Fixpoint extRen_PTm (xi_PTm : nat -> nat) (zeta_PTm : nat -> nat)
+(Eq_PTm : forall x, xi_PTm x = zeta_PTm x) (s : PTm) {struct s} :
 ren_PTm xi_PTm s = ren_PTm zeta_PTm s :=
   match s with
-  | VarPTm _ s0 => ap (VarPTm n_PTm) (Eq_PTm s0)
-  | PAbs _ s0 =>
+  | VarPTm s0 => ap (VarPTm) (Eq_PTm s0)
+  | PAbs s0 =>
       congr_PAbs
         (extRen_PTm (upRen_PTm_PTm xi_PTm) (upRen_PTm_PTm zeta_PTm)
            (upExtRen_PTm_PTm _ _ Eq_PTm) s0)
-  | PApp _ s0 s1 =>
+  | PApp s0 s1 =>
       congr_PApp (extRen_PTm xi_PTm zeta_PTm Eq_PTm s0)
         (extRen_PTm xi_PTm zeta_PTm Eq_PTm s1)
-  | PPair _ s0 s1 =>
+  | PPair s0 s1 =>
       congr_PPair (extRen_PTm xi_PTm zeta_PTm Eq_PTm s0)
         (extRen_PTm xi_PTm zeta_PTm Eq_PTm s1)
-  | PProj _ s0 s1 =>
+  | PProj s0 s1 =>
       congr_PProj (eq_refl s0) (extRen_PTm xi_PTm zeta_PTm Eq_PTm s1)
-  | PBind _ s0 s1 s2 =>
+  | PBind s0 s1 s2 =>
       congr_PBind (eq_refl s0) (extRen_PTm xi_PTm zeta_PTm Eq_PTm s1)
         (extRen_PTm (upRen_PTm_PTm xi_PTm) (upRen_PTm_PTm zeta_PTm)
            (upExtRen_PTm_PTm _ _ Eq_PTm) s2)
-  | PUniv _ s0 => congr_PUniv (eq_refl s0)
-  | PBot _ => congr_PBot
-  | PNat _ => congr_PNat
-  | PZero _ => congr_PZero
-  | PSuc _ s0 => congr_PSuc (extRen_PTm xi_PTm zeta_PTm Eq_PTm s0)
-  | PInd _ s0 s1 s2 s3 =>
+  | PUniv s0 => congr_PUniv (eq_refl s0)
+  | PBot => congr_PBot
+  | PNat => congr_PNat
+  | PZero => congr_PZero
+  | PSuc s0 => congr_PSuc (extRen_PTm xi_PTm zeta_PTm Eq_PTm s0)
+  | PInd s0 s1 s2 s3 =>
       congr_PInd
         (extRen_PTm (upRen_PTm_PTm xi_PTm) (upRen_PTm_PTm zeta_PTm)
            (upExtRen_PTm_PTm _ _ Eq_PTm) s0)
@@ -313,55 +258,44 @@ ren_PTm xi_PTm s = ren_PTm zeta_PTm s :=
            (upExtRen_PTm_PTm _ _ (upExtRen_PTm_PTm _ _ Eq_PTm)) s3)
   end.
 
-Lemma upExt_PTm_PTm {m : nat} {n_PTm : nat} (sigma : fin m -> PTm n_PTm)
-  (tau : fin m -> PTm n_PTm) (Eq : forall x, sigma x = tau x) :
+Lemma upExt_PTm_PTm (sigma : nat -> PTm) (tau : nat -> PTm)
+  (Eq : forall x, sigma x = tau x) :
   forall x, up_PTm_PTm sigma x = up_PTm_PTm tau x.
 Proof.
 exact (fun n =>
        match n with
-       | Some fin_n => ap (ren_PTm shift) (Eq fin_n)
-       | None => eq_refl
+       | S n' => ap (ren_PTm shift) (Eq n')
+       | O => eq_refl
        end).
 Qed.
 
-Lemma upExt_list_PTm_PTm {p : nat} {m : nat} {n_PTm : nat}
-  (sigma : fin m -> PTm n_PTm) (tau : fin m -> PTm n_PTm)
-  (Eq : forall x, sigma x = tau x) :
-  forall x, up_list_PTm_PTm p sigma x = up_list_PTm_PTm p tau x.
-Proof.
-exact (fun n =>
-       scons_p_congr (fun n => eq_refl)
-         (fun n => ap (ren_PTm (shift_p p)) (Eq n))).
-Qed.
-
-Fixpoint ext_PTm {m_PTm : nat} {n_PTm : nat}
-(sigma_PTm : fin m_PTm -> PTm n_PTm) (tau_PTm : fin m_PTm -> PTm n_PTm)
-(Eq_PTm : forall x, sigma_PTm x = tau_PTm x) (s : PTm m_PTm) {struct s} :
+Fixpoint ext_PTm (sigma_PTm : nat -> PTm) (tau_PTm : nat -> PTm)
+(Eq_PTm : forall x, sigma_PTm x = tau_PTm x) (s : PTm) {struct s} :
 subst_PTm sigma_PTm s = subst_PTm tau_PTm s :=
   match s with
-  | VarPTm _ s0 => Eq_PTm s0
-  | PAbs _ s0 =>
+  | VarPTm s0 => Eq_PTm s0
+  | PAbs s0 =>
       congr_PAbs
         (ext_PTm (up_PTm_PTm sigma_PTm) (up_PTm_PTm tau_PTm)
            (upExt_PTm_PTm _ _ Eq_PTm) s0)
-  | PApp _ s0 s1 =>
+  | PApp s0 s1 =>
       congr_PApp (ext_PTm sigma_PTm tau_PTm Eq_PTm s0)
         (ext_PTm sigma_PTm tau_PTm Eq_PTm s1)
-  | PPair _ s0 s1 =>
+  | PPair s0 s1 =>
       congr_PPair (ext_PTm sigma_PTm tau_PTm Eq_PTm s0)
         (ext_PTm sigma_PTm tau_PTm Eq_PTm s1)
-  | PProj _ s0 s1 =>
+  | PProj s0 s1 =>
       congr_PProj (eq_refl s0) (ext_PTm sigma_PTm tau_PTm Eq_PTm s1)
-  | PBind _ s0 s1 s2 =>
+  | PBind s0 s1 s2 =>
       congr_PBind (eq_refl s0) (ext_PTm sigma_PTm tau_PTm Eq_PTm s1)
         (ext_PTm (up_PTm_PTm sigma_PTm) (up_PTm_PTm tau_PTm)
            (upExt_PTm_PTm _ _ Eq_PTm) s2)
-  | PUniv _ s0 => congr_PUniv (eq_refl s0)
-  | PBot _ => congr_PBot
-  | PNat _ => congr_PNat
-  | PZero _ => congr_PZero
-  | PSuc _ s0 => congr_PSuc (ext_PTm sigma_PTm tau_PTm Eq_PTm s0)
-  | PInd _ s0 s1 s2 s3 =>
+  | PUniv s0 => congr_PUniv (eq_refl s0)
+  | PBot => congr_PBot
+  | PNat => congr_PNat
+  | PZero => congr_PZero
+  | PSuc s0 => congr_PSuc (ext_PTm sigma_PTm tau_PTm Eq_PTm s0)
+  | PInd s0 s1 s2 s3 =>
       congr_PInd
         (ext_PTm (up_PTm_PTm sigma_PTm) (up_PTm_PTm tau_PTm)
            (upExt_PTm_PTm _ _ Eq_PTm) s0)
@@ -372,57 +306,44 @@ subst_PTm sigma_PTm s = subst_PTm tau_PTm s :=
            (upExt_PTm_PTm _ _ (upExt_PTm_PTm _ _ Eq_PTm)) s3)
   end.
 
-Lemma up_ren_ren_PTm_PTm {k : nat} {l : nat} {m : nat} (xi : fin k -> fin l)
-  (zeta : fin l -> fin m) (rho : fin k -> fin m)
-  (Eq : forall x, funcomp zeta xi x = rho x) :
+Lemma up_ren_ren_PTm_PTm (xi : nat -> nat) (zeta : nat -> nat)
+  (rho : nat -> nat) (Eq : forall x, funcomp zeta xi x = rho x) :
   forall x,
   funcomp (upRen_PTm_PTm zeta) (upRen_PTm_PTm xi) x = upRen_PTm_PTm rho x.
 Proof.
 exact (up_ren_ren xi zeta rho Eq).
 Qed.
 
-Lemma up_ren_ren_list_PTm_PTm {p : nat} {k : nat} {l : nat} {m : nat}
-  (xi : fin k -> fin l) (zeta : fin l -> fin m) (rho : fin k -> fin m)
-  (Eq : forall x, funcomp zeta xi x = rho x) :
-  forall x,
-  funcomp (upRen_list_PTm_PTm p zeta) (upRen_list_PTm_PTm p xi) x =
-  upRen_list_PTm_PTm p rho x.
-Proof.
-exact (up_ren_ren_p Eq).
-Qed.
-
-Fixpoint compRenRen_PTm {k_PTm : nat} {l_PTm : nat} {m_PTm : nat}
-(xi_PTm : fin m_PTm -> fin k_PTm) (zeta_PTm : fin k_PTm -> fin l_PTm)
-(rho_PTm : fin m_PTm -> fin l_PTm)
-(Eq_PTm : forall x, funcomp zeta_PTm xi_PTm x = rho_PTm x) (s : PTm m_PTm)
-{struct s} : ren_PTm zeta_PTm (ren_PTm xi_PTm s) = ren_PTm rho_PTm s :=
+Fixpoint compRenRen_PTm (xi_PTm : nat -> nat) (zeta_PTm : nat -> nat)
+(rho_PTm : nat -> nat)
+(Eq_PTm : forall x, funcomp zeta_PTm xi_PTm x = rho_PTm x) (s : PTm) {struct
+ s} : ren_PTm zeta_PTm (ren_PTm xi_PTm s) = ren_PTm rho_PTm s :=
   match s with
-  | VarPTm _ s0 => ap (VarPTm l_PTm) (Eq_PTm s0)
-  | PAbs _ s0 =>
+  | VarPTm s0 => ap (VarPTm) (Eq_PTm s0)
+  | PAbs s0 =>
       congr_PAbs
         (compRenRen_PTm (upRen_PTm_PTm xi_PTm) (upRen_PTm_PTm zeta_PTm)
            (upRen_PTm_PTm rho_PTm) (up_ren_ren _ _ _ Eq_PTm) s0)
-  | PApp _ s0 s1 =>
+  | PApp s0 s1 =>
       congr_PApp (compRenRen_PTm xi_PTm zeta_PTm rho_PTm Eq_PTm s0)
         (compRenRen_PTm xi_PTm zeta_PTm rho_PTm Eq_PTm s1)
-  | PPair _ s0 s1 =>
+  | PPair s0 s1 =>
       congr_PPair (compRenRen_PTm xi_PTm zeta_PTm rho_PTm Eq_PTm s0)
         (compRenRen_PTm xi_PTm zeta_PTm rho_PTm Eq_PTm s1)
-  | PProj _ s0 s1 =>
+  | PProj s0 s1 =>
       congr_PProj (eq_refl s0)
         (compRenRen_PTm xi_PTm zeta_PTm rho_PTm Eq_PTm s1)
-  | PBind _ s0 s1 s2 =>
+  | PBind s0 s1 s2 =>
       congr_PBind (eq_refl s0)
         (compRenRen_PTm xi_PTm zeta_PTm rho_PTm Eq_PTm s1)
         (compRenRen_PTm (upRen_PTm_PTm xi_PTm) (upRen_PTm_PTm zeta_PTm)
            (upRen_PTm_PTm rho_PTm) (up_ren_ren _ _ _ Eq_PTm) s2)
-  | PUniv _ s0 => congr_PUniv (eq_refl s0)
-  | PBot _ => congr_PBot
-  | PNat _ => congr_PNat
-  | PZero _ => congr_PZero
-  | PSuc _ s0 =>
-      congr_PSuc (compRenRen_PTm xi_PTm zeta_PTm rho_PTm Eq_PTm s0)
-  | PInd _ s0 s1 s2 s3 =>
+  | PUniv s0 => congr_PUniv (eq_refl s0)
+  | PBot => congr_PBot
+  | PNat => congr_PNat
+  | PZero => congr_PZero
+  | PSuc s0 => congr_PSuc (compRenRen_PTm xi_PTm zeta_PTm rho_PTm Eq_PTm s0)
+  | PInd s0 s1 s2 s3 =>
       congr_PInd
         (compRenRen_PTm (upRen_PTm_PTm xi_PTm) (upRen_PTm_PTm zeta_PTm)
            (upRen_PTm_PTm rho_PTm) (up_ren_ren _ _ _ Eq_PTm) s0)
@@ -434,66 +355,49 @@ Fixpoint compRenRen_PTm {k_PTm : nat} {l_PTm : nat} {m_PTm : nat}
            (up_ren_ren _ _ _ (up_ren_ren _ _ _ Eq_PTm)) s3)
   end.
 
-Lemma up_ren_subst_PTm_PTm {k : nat} {l : nat} {m_PTm : nat}
-  (xi : fin k -> fin l) (tau : fin l -> PTm m_PTm)
-  (theta : fin k -> PTm m_PTm) (Eq : forall x, funcomp tau xi x = theta x) :
+Lemma up_ren_subst_PTm_PTm (xi : nat -> nat) (tau : nat -> PTm)
+  (theta : nat -> PTm) (Eq : forall x, funcomp tau xi x = theta x) :
   forall x,
   funcomp (up_PTm_PTm tau) (upRen_PTm_PTm xi) x = up_PTm_PTm theta x.
 Proof.
 exact (fun n =>
        match n with
-       | Some fin_n => ap (ren_PTm shift) (Eq fin_n)
-       | None => eq_refl
+       | S n' => ap (ren_PTm shift) (Eq n')
+       | O => eq_refl
        end).
 Qed.
 
-Lemma up_ren_subst_list_PTm_PTm {p : nat} {k : nat} {l : nat} {m_PTm : nat}
-  (xi : fin k -> fin l) (tau : fin l -> PTm m_PTm)
-  (theta : fin k -> PTm m_PTm) (Eq : forall x, funcomp tau xi x = theta x) :
-  forall x,
-  funcomp (up_list_PTm_PTm p tau) (upRen_list_PTm_PTm p xi) x =
-  up_list_PTm_PTm p theta x.
-Proof.
-exact (fun n =>
-       eq_trans (scons_p_comp' _ _ _ n)
-         (scons_p_congr (fun z => scons_p_head' _ _ z)
-            (fun z =>
-             eq_trans (scons_p_tail' _ _ (xi z))
-               (ap (ren_PTm (shift_p p)) (Eq z))))).
-Qed.
-
-Fixpoint compRenSubst_PTm {k_PTm : nat} {l_PTm : nat} {m_PTm : nat}
-(xi_PTm : fin m_PTm -> fin k_PTm) (tau_PTm : fin k_PTm -> PTm l_PTm)
-(theta_PTm : fin m_PTm -> PTm l_PTm)
-(Eq_PTm : forall x, funcomp tau_PTm xi_PTm x = theta_PTm x) (s : PTm m_PTm)
-{struct s} : subst_PTm tau_PTm (ren_PTm xi_PTm s) = subst_PTm theta_PTm s :=
+Fixpoint compRenSubst_PTm (xi_PTm : nat -> nat) (tau_PTm : nat -> PTm)
+(theta_PTm : nat -> PTm)
+(Eq_PTm : forall x, funcomp tau_PTm xi_PTm x = theta_PTm x) (s : PTm) {struct
+ s} : subst_PTm tau_PTm (ren_PTm xi_PTm s) = subst_PTm theta_PTm s :=
   match s with
-  | VarPTm _ s0 => Eq_PTm s0
-  | PAbs _ s0 =>
+  | VarPTm s0 => Eq_PTm s0
+  | PAbs s0 =>
       congr_PAbs
         (compRenSubst_PTm (upRen_PTm_PTm xi_PTm) (up_PTm_PTm tau_PTm)
            (up_PTm_PTm theta_PTm) (up_ren_subst_PTm_PTm _ _ _ Eq_PTm) s0)
-  | PApp _ s0 s1 =>
+  | PApp s0 s1 =>
       congr_PApp (compRenSubst_PTm xi_PTm tau_PTm theta_PTm Eq_PTm s0)
         (compRenSubst_PTm xi_PTm tau_PTm theta_PTm Eq_PTm s1)
-  | PPair _ s0 s1 =>
+  | PPair s0 s1 =>
       congr_PPair (compRenSubst_PTm xi_PTm tau_PTm theta_PTm Eq_PTm s0)
         (compRenSubst_PTm xi_PTm tau_PTm theta_PTm Eq_PTm s1)
-  | PProj _ s0 s1 =>
+  | PProj s0 s1 =>
       congr_PProj (eq_refl s0)
         (compRenSubst_PTm xi_PTm tau_PTm theta_PTm Eq_PTm s1)
-  | PBind _ s0 s1 s2 =>
+  | PBind s0 s1 s2 =>
       congr_PBind (eq_refl s0)
         (compRenSubst_PTm xi_PTm tau_PTm theta_PTm Eq_PTm s1)
         (compRenSubst_PTm (upRen_PTm_PTm xi_PTm) (up_PTm_PTm tau_PTm)
            (up_PTm_PTm theta_PTm) (up_ren_subst_PTm_PTm _ _ _ Eq_PTm) s2)
-  | PUniv _ s0 => congr_PUniv (eq_refl s0)
-  | PBot _ => congr_PBot
-  | PNat _ => congr_PNat
-  | PZero _ => congr_PZero
-  | PSuc _ s0 =>
+  | PUniv s0 => congr_PUniv (eq_refl s0)
+  | PBot => congr_PBot
+  | PNat => congr_PNat
+  | PZero => congr_PZero
+  | PSuc s0 =>
       congr_PSuc (compRenSubst_PTm xi_PTm tau_PTm theta_PTm Eq_PTm s0)
-  | PInd _ s0 s1 s2 s3 =>
+  | PInd s0 s1 s2 s3 =>
       congr_PInd
         (compRenSubst_PTm (upRen_PTm_PTm xi_PTm) (up_PTm_PTm tau_PTm)
            (up_PTm_PTm theta_PTm) (up_ren_subst_PTm_PTm _ _ _ Eq_PTm) s0)
@@ -506,9 +410,8 @@ Fixpoint compRenSubst_PTm {k_PTm : nat} {l_PTm : nat} {m_PTm : nat}
            s3)
   end.
 
-Lemma up_subst_ren_PTm_PTm {k : nat} {l_PTm : nat} {m_PTm : nat}
-  (sigma : fin k -> PTm l_PTm) (zeta_PTm : fin l_PTm -> fin m_PTm)
-  (theta : fin k -> PTm m_PTm)
+Lemma up_subst_ren_PTm_PTm (sigma : nat -> PTm) (zeta_PTm : nat -> nat)
+  (theta : nat -> PTm)
   (Eq : forall x, funcomp (ren_PTm zeta_PTm) sigma x = theta x) :
   forall x,
   funcomp (ren_PTm (upRen_PTm_PTm zeta_PTm)) (up_PTm_PTm sigma) x =
@@ -516,76 +419,51 @@ Lemma up_subst_ren_PTm_PTm {k : nat} {l_PTm : nat} {m_PTm : nat}
 Proof.
 exact (fun n =>
        match n with
-       | Some fin_n =>
+       | S n' =>
            eq_trans
              (compRenRen_PTm shift (upRen_PTm_PTm zeta_PTm)
-                (funcomp shift zeta_PTm) (fun x => eq_refl) (sigma fin_n))
+                (funcomp shift zeta_PTm) (fun x => eq_refl) (sigma n'))
              (eq_trans
                 (eq_sym
                    (compRenRen_PTm zeta_PTm shift (funcomp shift zeta_PTm)
-                      (fun x => eq_refl) (sigma fin_n)))
-                (ap (ren_PTm shift) (Eq fin_n)))
-       | None => eq_refl
+                      (fun x => eq_refl) (sigma n')))
+                (ap (ren_PTm shift) (Eq n')))
+       | O => eq_refl
        end).
 Qed.
 
-Lemma up_subst_ren_list_PTm_PTm {p : nat} {k : nat} {l_PTm : nat}
-  {m_PTm : nat} (sigma : fin k -> PTm l_PTm)
-  (zeta_PTm : fin l_PTm -> fin m_PTm) (theta : fin k -> PTm m_PTm)
-  (Eq : forall x, funcomp (ren_PTm zeta_PTm) sigma x = theta x) :
-  forall x,
-  funcomp (ren_PTm (upRen_list_PTm_PTm p zeta_PTm)) (up_list_PTm_PTm p sigma)
-    x = up_list_PTm_PTm p theta x.
-Proof.
-exact (fun n =>
-       eq_trans (scons_p_comp' _ _ _ n)
-         (scons_p_congr
-            (fun x => ap (VarPTm (plus p m_PTm)) (scons_p_head' _ _ x))
-            (fun n =>
-             eq_trans
-               (compRenRen_PTm (shift_p p) (upRen_list_PTm_PTm p zeta_PTm)
-                  (funcomp (shift_p p) zeta_PTm)
-                  (fun x => scons_p_tail' _ _ x) (sigma n))
-               (eq_trans
-                  (eq_sym
-                     (compRenRen_PTm zeta_PTm (shift_p p)
-                        (funcomp (shift_p p) zeta_PTm) (fun x => eq_refl)
-                        (sigma n))) (ap (ren_PTm (shift_p p)) (Eq n)))))).
-Qed.
-
-Fixpoint compSubstRen_PTm {k_PTm : nat} {l_PTm : nat} {m_PTm : nat}
-(sigma_PTm : fin m_PTm -> PTm k_PTm) (zeta_PTm : fin k_PTm -> fin l_PTm)
-(theta_PTm : fin m_PTm -> PTm l_PTm)
+Fixpoint compSubstRen_PTm (sigma_PTm : nat -> PTm) (zeta_PTm : nat -> nat)
+(theta_PTm : nat -> PTm)
 (Eq_PTm : forall x, funcomp (ren_PTm zeta_PTm) sigma_PTm x = theta_PTm x)
-(s : PTm m_PTm) {struct s} :
+(s : PTm) {struct s} :
 ren_PTm zeta_PTm (subst_PTm sigma_PTm s) = subst_PTm theta_PTm s :=
   match s with
-  | VarPTm _ s0 => Eq_PTm s0
-  | PAbs _ s0 =>
+  | VarPTm s0 => Eq_PTm s0
+  | PAbs s0 =>
       congr_PAbs
         (compSubstRen_PTm (up_PTm_PTm sigma_PTm) (upRen_PTm_PTm zeta_PTm)
            (up_PTm_PTm theta_PTm) (up_subst_ren_PTm_PTm _ _ _ Eq_PTm) s0)
-  | PApp _ s0 s1 =>
+  | PApp s0 s1 =>
       congr_PApp (compSubstRen_PTm sigma_PTm zeta_PTm theta_PTm Eq_PTm s0)
         (compSubstRen_PTm sigma_PTm zeta_PTm theta_PTm Eq_PTm s1)
-  | PPair _ s0 s1 =>
+  | PPair s0 s1 =>
       congr_PPair (compSubstRen_PTm sigma_PTm zeta_PTm theta_PTm Eq_PTm s0)
         (compSubstRen_PTm sigma_PTm zeta_PTm theta_PTm Eq_PTm s1)
-  | PProj _ s0 s1 =>
+  | PProj s0 s1 =>
       congr_PProj (eq_refl s0)
         (compSubstRen_PTm sigma_PTm zeta_PTm theta_PTm Eq_PTm s1)
-  | PBind _ s0 s1 s2 =>
+  | PBind s0 s1 s2 =>
       congr_PBind (eq_refl s0)
         (compSubstRen_PTm sigma_PTm zeta_PTm theta_PTm Eq_PTm s1)
         (compSubstRen_PTm (up_PTm_PTm sigma_PTm) (upRen_PTm_PTm zeta_PTm)
            (up_PTm_PTm theta_PTm) (up_subst_ren_PTm_PTm _ _ _ Eq_PTm) s2)
-  | PUniv _ s0 => congr_PUniv (eq_refl s0)
-  | PBot _ => congr_PBot
-  | PNat _ => congr_PNat
-  | PZero _ => congr_PZero
-  | PSuc _ s0 =>
+  | PUniv s0 => congr_PUniv (eq_refl s0)
+  | PBot => congr_PBot
+  | PNat => congr_PNat
+  | PZero => congr_PZero
+  | PSuc s0 =>
       congr_PSuc (compSubstRen_PTm sigma_PTm zeta_PTm theta_PTm Eq_PTm s0)
-  | PInd _ s0 s1 s2 s3 =>
+  | PInd s0 s1 s2 s3 =>
       congr_PInd
         (compSubstRen_PTm (up_PTm_PTm sigma_PTm) (upRen_PTm_PTm zeta_PTm)
            (up_PTm_PTm theta_PTm) (up_subst_ren_PTm_PTm _ _ _ Eq_PTm) s0)
@@ -598,9 +476,8 @@ ren_PTm zeta_PTm (subst_PTm sigma_PTm s) = subst_PTm theta_PTm s :=
            s3)
   end.
 
-Lemma up_subst_subst_PTm_PTm {k : nat} {l_PTm : nat} {m_PTm : nat}
-  (sigma : fin k -> PTm l_PTm) (tau_PTm : fin l_PTm -> PTm m_PTm)
-  (theta : fin k -> PTm m_PTm)
+Lemma up_subst_subst_PTm_PTm (sigma : nat -> PTm) (tau_PTm : nat -> PTm)
+  (theta : nat -> PTm)
   (Eq : forall x, funcomp (subst_PTm tau_PTm) sigma x = theta x) :
   forall x,
   funcomp (subst_PTm (up_PTm_PTm tau_PTm)) (up_PTm_PTm sigma) x =
@@ -608,78 +485,52 @@ Lemma up_subst_subst_PTm_PTm {k : nat} {l_PTm : nat} {m_PTm : nat}
 Proof.
 exact (fun n =>
        match n with
-       | Some fin_n =>
+       | S n' =>
            eq_trans
              (compRenSubst_PTm shift (up_PTm_PTm tau_PTm)
                 (funcomp (up_PTm_PTm tau_PTm) shift) (fun x => eq_refl)
-                (sigma fin_n))
+                (sigma n'))
              (eq_trans
                 (eq_sym
                    (compSubstRen_PTm tau_PTm shift
                       (funcomp (ren_PTm shift) tau_PTm) (fun x => eq_refl)
-                      (sigma fin_n))) (ap (ren_PTm shift) (Eq fin_n)))
-       | None => eq_refl
+                      (sigma n'))) (ap (ren_PTm shift) (Eq n')))
+       | O => eq_refl
        end).
 Qed.
 
-Lemma up_subst_subst_list_PTm_PTm {p : nat} {k : nat} {l_PTm : nat}
-  {m_PTm : nat} (sigma : fin k -> PTm l_PTm)
-  (tau_PTm : fin l_PTm -> PTm m_PTm) (theta : fin k -> PTm m_PTm)
-  (Eq : forall x, funcomp (subst_PTm tau_PTm) sigma x = theta x) :
-  forall x,
-  funcomp (subst_PTm (up_list_PTm_PTm p tau_PTm)) (up_list_PTm_PTm p sigma) x =
-  up_list_PTm_PTm p theta x.
-Proof.
-exact (fun n =>
-       eq_trans
-         (scons_p_comp' (funcomp (VarPTm (plus p l_PTm)) (zero_p p)) _ _ n)
-         (scons_p_congr
-            (fun x => scons_p_head' _ (fun z => ren_PTm (shift_p p) _) x)
-            (fun n =>
-             eq_trans
-               (compRenSubst_PTm (shift_p p) (up_list_PTm_PTm p tau_PTm)
-                  (funcomp (up_list_PTm_PTm p tau_PTm) (shift_p p))
-                  (fun x => eq_refl) (sigma n))
-               (eq_trans
-                  (eq_sym
-                     (compSubstRen_PTm tau_PTm (shift_p p) _
-                        (fun x => eq_sym (scons_p_tail' _ _ x)) (sigma n)))
-                  (ap (ren_PTm (shift_p p)) (Eq n)))))).
-Qed.
-
-Fixpoint compSubstSubst_PTm {k_PTm : nat} {l_PTm : nat} {m_PTm : nat}
-(sigma_PTm : fin m_PTm -> PTm k_PTm) (tau_PTm : fin k_PTm -> PTm l_PTm)
-(theta_PTm : fin m_PTm -> PTm l_PTm)
+Fixpoint compSubstSubst_PTm (sigma_PTm : nat -> PTm) (tau_PTm : nat -> PTm)
+(theta_PTm : nat -> PTm)
 (Eq_PTm : forall x, funcomp (subst_PTm tau_PTm) sigma_PTm x = theta_PTm x)
-(s : PTm m_PTm) {struct s} :
+(s : PTm) {struct s} :
 subst_PTm tau_PTm (subst_PTm sigma_PTm s) = subst_PTm theta_PTm s :=
   match s with
-  | VarPTm _ s0 => Eq_PTm s0
-  | PAbs _ s0 =>
+  | VarPTm s0 => Eq_PTm s0
+  | PAbs s0 =>
       congr_PAbs
         (compSubstSubst_PTm (up_PTm_PTm sigma_PTm) (up_PTm_PTm tau_PTm)
            (up_PTm_PTm theta_PTm) (up_subst_subst_PTm_PTm _ _ _ Eq_PTm) s0)
-  | PApp _ s0 s1 =>
+  | PApp s0 s1 =>
       congr_PApp (compSubstSubst_PTm sigma_PTm tau_PTm theta_PTm Eq_PTm s0)
         (compSubstSubst_PTm sigma_PTm tau_PTm theta_PTm Eq_PTm s1)
-  | PPair _ s0 s1 =>
+  | PPair s0 s1 =>
       congr_PPair (compSubstSubst_PTm sigma_PTm tau_PTm theta_PTm Eq_PTm s0)
         (compSubstSubst_PTm sigma_PTm tau_PTm theta_PTm Eq_PTm s1)
-  | PProj _ s0 s1 =>
+  | PProj s0 s1 =>
       congr_PProj (eq_refl s0)
         (compSubstSubst_PTm sigma_PTm tau_PTm theta_PTm Eq_PTm s1)
-  | PBind _ s0 s1 s2 =>
+  | PBind s0 s1 s2 =>
       congr_PBind (eq_refl s0)
         (compSubstSubst_PTm sigma_PTm tau_PTm theta_PTm Eq_PTm s1)
         (compSubstSubst_PTm (up_PTm_PTm sigma_PTm) (up_PTm_PTm tau_PTm)
            (up_PTm_PTm theta_PTm) (up_subst_subst_PTm_PTm _ _ _ Eq_PTm) s2)
-  | PUniv _ s0 => congr_PUniv (eq_refl s0)
-  | PBot _ => congr_PBot
-  | PNat _ => congr_PNat
-  | PZero _ => congr_PZero
-  | PSuc _ s0 =>
+  | PUniv s0 => congr_PUniv (eq_refl s0)
+  | PBot => congr_PBot
+  | PNat => congr_PNat
+  | PZero => congr_PZero
+  | PSuc s0 =>
       congr_PSuc (compSubstSubst_PTm sigma_PTm tau_PTm theta_PTm Eq_PTm s0)
-  | PInd _ s0 s1 s2 s3 =>
+  | PInd s0 s1 s2 s3 =>
       congr_PInd
         (compSubstSubst_PTm (up_PTm_PTm sigma_PTm) (up_PTm_PTm tau_PTm)
            (up_PTm_PTm theta_PTm) (up_subst_subst_PTm_PTm _ _ _ Eq_PTm) s0)
@@ -692,126 +543,102 @@ subst_PTm tau_PTm (subst_PTm sigma_PTm s) = subst_PTm theta_PTm s :=
               (up_subst_subst_PTm_PTm _ _ _ Eq_PTm)) s3)
   end.
 
-Lemma renRen_PTm {k_PTm : nat} {l_PTm : nat} {m_PTm : nat}
-  (xi_PTm : fin m_PTm -> fin k_PTm) (zeta_PTm : fin k_PTm -> fin l_PTm)
-  (s : PTm m_PTm) :
+Lemma renRen_PTm (xi_PTm : nat -> nat) (zeta_PTm : nat -> nat) (s : PTm) :
   ren_PTm zeta_PTm (ren_PTm xi_PTm s) = ren_PTm (funcomp zeta_PTm xi_PTm) s.
 Proof.
 exact (compRenRen_PTm xi_PTm zeta_PTm _ (fun n => eq_refl) s).
 Qed.
 
-Lemma renRen'_PTm_pointwise {k_PTm : nat} {l_PTm : nat} {m_PTm : nat}
-  (xi_PTm : fin m_PTm -> fin k_PTm) (zeta_PTm : fin k_PTm -> fin l_PTm) :
+Lemma renRen'_PTm_pointwise (xi_PTm : nat -> nat) (zeta_PTm : nat -> nat) :
   pointwise_relation _ eq (funcomp (ren_PTm zeta_PTm) (ren_PTm xi_PTm))
     (ren_PTm (funcomp zeta_PTm xi_PTm)).
 Proof.
 exact (fun s => compRenRen_PTm xi_PTm zeta_PTm _ (fun n => eq_refl) s).
 Qed.
 
-Lemma renSubst_PTm {k_PTm : nat} {l_PTm : nat} {m_PTm : nat}
-  (xi_PTm : fin m_PTm -> fin k_PTm) (tau_PTm : fin k_PTm -> PTm l_PTm)
-  (s : PTm m_PTm) :
+Lemma renSubst_PTm (xi_PTm : nat -> nat) (tau_PTm : nat -> PTm) (s : PTm) :
   subst_PTm tau_PTm (ren_PTm xi_PTm s) = subst_PTm (funcomp tau_PTm xi_PTm) s.
 Proof.
 exact (compRenSubst_PTm xi_PTm tau_PTm _ (fun n => eq_refl) s).
 Qed.
 
-Lemma renSubst_PTm_pointwise {k_PTm : nat} {l_PTm : nat} {m_PTm : nat}
-  (xi_PTm : fin m_PTm -> fin k_PTm) (tau_PTm : fin k_PTm -> PTm l_PTm) :
+Lemma renSubst_PTm_pointwise (xi_PTm : nat -> nat) (tau_PTm : nat -> PTm) :
   pointwise_relation _ eq (funcomp (subst_PTm tau_PTm) (ren_PTm xi_PTm))
     (subst_PTm (funcomp tau_PTm xi_PTm)).
 Proof.
 exact (fun s => compRenSubst_PTm xi_PTm tau_PTm _ (fun n => eq_refl) s).
 Qed.
 
-Lemma substRen_PTm {k_PTm : nat} {l_PTm : nat} {m_PTm : nat}
-  (sigma_PTm : fin m_PTm -> PTm k_PTm) (zeta_PTm : fin k_PTm -> fin l_PTm)
-  (s : PTm m_PTm) :
+Lemma substRen_PTm (sigma_PTm : nat -> PTm) (zeta_PTm : nat -> nat) (s : PTm)
+  :
   ren_PTm zeta_PTm (subst_PTm sigma_PTm s) =
   subst_PTm (funcomp (ren_PTm zeta_PTm) sigma_PTm) s.
 Proof.
 exact (compSubstRen_PTm sigma_PTm zeta_PTm _ (fun n => eq_refl) s).
 Qed.
 
-Lemma substRen_PTm_pointwise {k_PTm : nat} {l_PTm : nat} {m_PTm : nat}
-  (sigma_PTm : fin m_PTm -> PTm k_PTm) (zeta_PTm : fin k_PTm -> fin l_PTm) :
+Lemma substRen_PTm_pointwise (sigma_PTm : nat -> PTm) (zeta_PTm : nat -> nat)
+  :
   pointwise_relation _ eq (funcomp (ren_PTm zeta_PTm) (subst_PTm sigma_PTm))
     (subst_PTm (funcomp (ren_PTm zeta_PTm) sigma_PTm)).
 Proof.
 exact (fun s => compSubstRen_PTm sigma_PTm zeta_PTm _ (fun n => eq_refl) s).
 Qed.
 
-Lemma substSubst_PTm {k_PTm : nat} {l_PTm : nat} {m_PTm : nat}
-  (sigma_PTm : fin m_PTm -> PTm k_PTm) (tau_PTm : fin k_PTm -> PTm l_PTm)
-  (s : PTm m_PTm) :
+Lemma substSubst_PTm (sigma_PTm : nat -> PTm) (tau_PTm : nat -> PTm)
+  (s : PTm) :
   subst_PTm tau_PTm (subst_PTm sigma_PTm s) =
   subst_PTm (funcomp (subst_PTm tau_PTm) sigma_PTm) s.
 Proof.
 exact (compSubstSubst_PTm sigma_PTm tau_PTm _ (fun n => eq_refl) s).
 Qed.
 
-Lemma substSubst_PTm_pointwise {k_PTm : nat} {l_PTm : nat} {m_PTm : nat}
-  (sigma_PTm : fin m_PTm -> PTm k_PTm) (tau_PTm : fin k_PTm -> PTm l_PTm) :
+Lemma substSubst_PTm_pointwise (sigma_PTm : nat -> PTm)
+  (tau_PTm : nat -> PTm) :
   pointwise_relation _ eq (funcomp (subst_PTm tau_PTm) (subst_PTm sigma_PTm))
     (subst_PTm (funcomp (subst_PTm tau_PTm) sigma_PTm)).
 Proof.
 exact (fun s => compSubstSubst_PTm sigma_PTm tau_PTm _ (fun n => eq_refl) s).
 Qed.
 
-Lemma rinstInst_up_PTm_PTm {m : nat} {n_PTm : nat} (xi : fin m -> fin n_PTm)
-  (sigma : fin m -> PTm n_PTm)
-  (Eq : forall x, funcomp (VarPTm n_PTm) xi x = sigma x) :
-  forall x,
-  funcomp (VarPTm (S n_PTm)) (upRen_PTm_PTm xi) x = up_PTm_PTm sigma x.
+Lemma rinstInst_up_PTm_PTm (xi : nat -> nat) (sigma : nat -> PTm)
+  (Eq : forall x, funcomp (VarPTm) xi x = sigma x) :
+  forall x, funcomp (VarPTm) (upRen_PTm_PTm xi) x = up_PTm_PTm sigma x.
 Proof.
 exact (fun n =>
        match n with
-       | Some fin_n => ap (ren_PTm shift) (Eq fin_n)
-       | None => eq_refl
+       | S n' => ap (ren_PTm shift) (Eq n')
+       | O => eq_refl
        end).
 Qed.
 
-Lemma rinstInst_up_list_PTm_PTm {p : nat} {m : nat} {n_PTm : nat}
-  (xi : fin m -> fin n_PTm) (sigma : fin m -> PTm n_PTm)
-  (Eq : forall x, funcomp (VarPTm n_PTm) xi x = sigma x) :
-  forall x,
-  funcomp (VarPTm (plus p n_PTm)) (upRen_list_PTm_PTm p xi) x =
-  up_list_PTm_PTm p sigma x.
-Proof.
-exact (fun n =>
-       eq_trans (scons_p_comp' _ _ (VarPTm (plus p n_PTm)) n)
-         (scons_p_congr (fun z => eq_refl)
-            (fun n => ap (ren_PTm (shift_p p)) (Eq n)))).
-Qed.
-
-Fixpoint rinst_inst_PTm {m_PTm : nat} {n_PTm : nat}
-(xi_PTm : fin m_PTm -> fin n_PTm) (sigma_PTm : fin m_PTm -> PTm n_PTm)
-(Eq_PTm : forall x, funcomp (VarPTm n_PTm) xi_PTm x = sigma_PTm x)
-(s : PTm m_PTm) {struct s} : ren_PTm xi_PTm s = subst_PTm sigma_PTm s :=
+Fixpoint rinst_inst_PTm (xi_PTm : nat -> nat) (sigma_PTm : nat -> PTm)
+(Eq_PTm : forall x, funcomp (VarPTm) xi_PTm x = sigma_PTm x) (s : PTm)
+{struct s} : ren_PTm xi_PTm s = subst_PTm sigma_PTm s :=
   match s with
-  | VarPTm _ s0 => Eq_PTm s0
-  | PAbs _ s0 =>
+  | VarPTm s0 => Eq_PTm s0
+  | PAbs s0 =>
       congr_PAbs
         (rinst_inst_PTm (upRen_PTm_PTm xi_PTm) (up_PTm_PTm sigma_PTm)
            (rinstInst_up_PTm_PTm _ _ Eq_PTm) s0)
-  | PApp _ s0 s1 =>
+  | PApp s0 s1 =>
       congr_PApp (rinst_inst_PTm xi_PTm sigma_PTm Eq_PTm s0)
         (rinst_inst_PTm xi_PTm sigma_PTm Eq_PTm s1)
-  | PPair _ s0 s1 =>
+  | PPair s0 s1 =>
       congr_PPair (rinst_inst_PTm xi_PTm sigma_PTm Eq_PTm s0)
         (rinst_inst_PTm xi_PTm sigma_PTm Eq_PTm s1)
-  | PProj _ s0 s1 =>
+  | PProj s0 s1 =>
       congr_PProj (eq_refl s0) (rinst_inst_PTm xi_PTm sigma_PTm Eq_PTm s1)
-  | PBind _ s0 s1 s2 =>
+  | PBind s0 s1 s2 =>
       congr_PBind (eq_refl s0) (rinst_inst_PTm xi_PTm sigma_PTm Eq_PTm s1)
         (rinst_inst_PTm (upRen_PTm_PTm xi_PTm) (up_PTm_PTm sigma_PTm)
            (rinstInst_up_PTm_PTm _ _ Eq_PTm) s2)
-  | PUniv _ s0 => congr_PUniv (eq_refl s0)
-  | PBot _ => congr_PBot
-  | PNat _ => congr_PNat
-  | PZero _ => congr_PZero
-  | PSuc _ s0 => congr_PSuc (rinst_inst_PTm xi_PTm sigma_PTm Eq_PTm s0)
-  | PInd _ s0 s1 s2 s3 =>
+  | PUniv s0 => congr_PUniv (eq_refl s0)
+  | PBot => congr_PBot
+  | PNat => congr_PNat
+  | PZero => congr_PZero
+  | PSuc s0 => congr_PSuc (rinst_inst_PTm xi_PTm sigma_PTm Eq_PTm s0)
+  | PInd s0 s1 s2 s3 =>
       congr_PInd
         (rinst_inst_PTm (upRen_PTm_PTm xi_PTm) (up_PTm_PTm sigma_PTm)
            (rinstInst_up_PTm_PTm _ _ Eq_PTm) s0)
@@ -822,71 +649,61 @@ Fixpoint rinst_inst_PTm {m_PTm : nat} {n_PTm : nat}
            (rinstInst_up_PTm_PTm _ _ (rinstInst_up_PTm_PTm _ _ Eq_PTm)) s3)
   end.
 
-Lemma rinstInst'_PTm {m_PTm : nat} {n_PTm : nat}
-  (xi_PTm : fin m_PTm -> fin n_PTm) (s : PTm m_PTm) :
-  ren_PTm xi_PTm s = subst_PTm (funcomp (VarPTm n_PTm) xi_PTm) s.
+Lemma rinstInst'_PTm (xi_PTm : nat -> nat) (s : PTm) :
+  ren_PTm xi_PTm s = subst_PTm (funcomp (VarPTm) xi_PTm) s.
 Proof.
 exact (rinst_inst_PTm xi_PTm _ (fun n => eq_refl) s).
 Qed.
 
-Lemma rinstInst'_PTm_pointwise {m_PTm : nat} {n_PTm : nat}
-  (xi_PTm : fin m_PTm -> fin n_PTm) :
+Lemma rinstInst'_PTm_pointwise (xi_PTm : nat -> nat) :
   pointwise_relation _ eq (ren_PTm xi_PTm)
-    (subst_PTm (funcomp (VarPTm n_PTm) xi_PTm)).
+    (subst_PTm (funcomp (VarPTm) xi_PTm)).
 Proof.
 exact (fun s => rinst_inst_PTm xi_PTm _ (fun n => eq_refl) s).
 Qed.
 
-Lemma instId'_PTm {m_PTm : nat} (s : PTm m_PTm) :
-  subst_PTm (VarPTm m_PTm) s = s.
+Lemma instId'_PTm (s : PTm) : subst_PTm (VarPTm) s = s.
 Proof.
-exact (idSubst_PTm (VarPTm m_PTm) (fun n => eq_refl) s).
+exact (idSubst_PTm (VarPTm) (fun n => eq_refl) s).
 Qed.
 
-Lemma instId'_PTm_pointwise {m_PTm : nat} :
-  pointwise_relation _ eq (subst_PTm (VarPTm m_PTm)) id.
+Lemma instId'_PTm_pointwise : pointwise_relation _ eq (subst_PTm (VarPTm)) id.
 Proof.
-exact (fun s => idSubst_PTm (VarPTm m_PTm) (fun n => eq_refl) s).
+exact (fun s => idSubst_PTm (VarPTm) (fun n => eq_refl) s).
 Qed.
 
-Lemma rinstId'_PTm {m_PTm : nat} (s : PTm m_PTm) : ren_PTm id s = s.
+Lemma rinstId'_PTm (s : PTm) : ren_PTm id s = s.
 Proof.
 exact (eq_ind_r (fun t => t = s) (instId'_PTm s) (rinstInst'_PTm id s)).
 Qed.
 
-Lemma rinstId'_PTm_pointwise {m_PTm : nat} :
-  pointwise_relation _ eq (@ren_PTm m_PTm m_PTm id) id.
+Lemma rinstId'_PTm_pointwise : pointwise_relation _ eq (@ren_PTm id) id.
 Proof.
 exact (fun s =>
        eq_ind_r (fun t => t = s) (instId'_PTm s) (rinstInst'_PTm id s)).
 Qed.
 
-Lemma varL'_PTm {m_PTm : nat} {n_PTm : nat}
-  (sigma_PTm : fin m_PTm -> PTm n_PTm) (x : fin m_PTm) :
-  subst_PTm sigma_PTm (VarPTm m_PTm x) = sigma_PTm x.
+Lemma varL'_PTm (sigma_PTm : nat -> PTm) (x : nat) :
+  subst_PTm sigma_PTm (VarPTm x) = sigma_PTm x.
 Proof.
 exact (eq_refl).
 Qed.
 
-Lemma varL'_PTm_pointwise {m_PTm : nat} {n_PTm : nat}
-  (sigma_PTm : fin m_PTm -> PTm n_PTm) :
-  pointwise_relation _ eq (funcomp (subst_PTm sigma_PTm) (VarPTm m_PTm))
-    sigma_PTm.
+Lemma varL'_PTm_pointwise (sigma_PTm : nat -> PTm) :
+  pointwise_relation _ eq (funcomp (subst_PTm sigma_PTm) (VarPTm)) sigma_PTm.
 Proof.
 exact (fun x => eq_refl).
 Qed.
 
-Lemma varLRen'_PTm {m_PTm : nat} {n_PTm : nat}
-  (xi_PTm : fin m_PTm -> fin n_PTm) (x : fin m_PTm) :
-  ren_PTm xi_PTm (VarPTm m_PTm x) = VarPTm n_PTm (xi_PTm x).
+Lemma varLRen'_PTm (xi_PTm : nat -> nat) (x : nat) :
+  ren_PTm xi_PTm (VarPTm x) = VarPTm (xi_PTm x).
 Proof.
 exact (eq_refl).
 Qed.
 
-Lemma varLRen'_PTm_pointwise {m_PTm : nat} {n_PTm : nat}
-  (xi_PTm : fin m_PTm -> fin n_PTm) :
-  pointwise_relation _ eq (funcomp (ren_PTm xi_PTm) (VarPTm m_PTm))
-    (funcomp (VarPTm n_PTm) xi_PTm).
+Lemma varLRen'_PTm_pointwise (xi_PTm : nat -> nat) :
+  pointwise_relation _ eq (funcomp (ren_PTm xi_PTm) (VarPTm))
+    (funcomp (VarPTm) xi_PTm).
 Proof.
 exact (fun x => eq_refl).
 Qed.
@@ -894,18 +711,14 @@ Qed.
 Class Up_PTm X Y :=
     up_PTm : X -> Y.
 
-#[global]
-Instance Subst_PTm  {m_PTm n_PTm : nat}: (Subst1 _ _ _) :=
- (@subst_PTm m_PTm n_PTm).
+#[global]Instance Subst_PTm : (Subst1 _ _ _) := @subst_PTm.
+
+#[global]Instance Up_PTm_PTm : (Up_PTm _ _) := @up_PTm_PTm.
+
+#[global]Instance Ren_PTm : (Ren1 _ _ _) := @ren_PTm.
 
 #[global]
-Instance Up_PTm_PTm  {m n_PTm : nat}: (Up_PTm _ _) := (@up_PTm_PTm m n_PTm).
-
-#[global]
-Instance Ren_PTm  {m_PTm n_PTm : nat}: (Ren1 _ _ _) := (@ren_PTm m_PTm n_PTm).
-
-#[global]
-Instance VarInstance_PTm  {n_PTm : nat}: (Var _ _) := (@VarPTm n_PTm).
+Instance VarInstance_PTm : (Var _ _) := @VarPTm.
 
 Notation "[ sigma_PTm ]" := (subst_PTm sigma_PTm)
 ( at level 1, left associativity, only printing)  : fscope.
@@ -932,9 +745,9 @@ Notation "x '__PTm'" := (VarPTm x) ( at level 5, format "x __PTm")  :
 subst_scope.
 
 #[global]
-Instance subst_PTm_morphism  {m_PTm : nat} {n_PTm : nat}:
+Instance subst_PTm_morphism :
  (Proper (respectful (pointwise_relation _ eq) (respectful eq eq))
-    (@subst_PTm m_PTm n_PTm)).
+    (@subst_PTm)).
 Proof.
 exact (fun f_PTm g_PTm Eq_PTm s t Eq_st =>
        eq_ind s (fun t' => subst_PTm f_PTm s = subst_PTm g_PTm t')
@@ -942,17 +755,16 @@ exact (fun f_PTm g_PTm Eq_PTm s t Eq_st =>
 Qed.
 
 #[global]
-Instance subst_PTm_morphism2  {m_PTm : nat} {n_PTm : nat}:
+Instance subst_PTm_morphism2 :
  (Proper (respectful (pointwise_relation _ eq) (pointwise_relation _ eq))
-    (@subst_PTm m_PTm n_PTm)).
+    (@subst_PTm)).
 Proof.
 exact (fun f_PTm g_PTm Eq_PTm s => ext_PTm f_PTm g_PTm Eq_PTm s).
 Qed.
 
 #[global]
-Instance ren_PTm_morphism  {m_PTm : nat} {n_PTm : nat}:
- (Proper (respectful (pointwise_relation _ eq) (respectful eq eq))
-    (@ren_PTm m_PTm n_PTm)).
+Instance ren_PTm_morphism :
+ (Proper (respectful (pointwise_relation _ eq) (respectful eq eq)) (@ren_PTm)).
 Proof.
 exact (fun f_PTm g_PTm Eq_PTm s t Eq_st =>
        eq_ind s (fun t' => ren_PTm f_PTm s = ren_PTm g_PTm t')
@@ -960,9 +772,9 @@ exact (fun f_PTm g_PTm Eq_PTm s t Eq_st =>
 Qed.
 
 #[global]
-Instance ren_PTm_morphism2  {m_PTm : nat} {n_PTm : nat}:
+Instance ren_PTm_morphism2 :
  (Proper (respectful (pointwise_relation _ eq) (pointwise_relation _ eq))
-    (@ren_PTm m_PTm n_PTm)).
+    (@ren_PTm)).
 Proof.
 exact (fun f_PTm g_PTm Eq_PTm s => extRen_PTm f_PTm g_PTm Eq_PTm s).
 Qed.
@@ -994,9 +806,7 @@ Ltac asimpl' := repeat (first
                  | progress setoid_rewrite rinstId'_PTm
                  | progress setoid_rewrite instId'_PTm_pointwise
                  | progress setoid_rewrite instId'_PTm
-                 | progress
-                    unfold up_list_PTm_PTm, up_PTm_PTm, upRen_list_PTm_PTm,
-                     upRen_PTm_PTm, up_ren
+                 | progress unfold up_PTm_PTm, upRen_PTm_PTm, up_ren
                  | progress cbn[subst_PTm ren_PTm]
                  | progress fsimpl ]).
 
@@ -1021,32 +831,7 @@ End Core.
 
 Module Extra.
 
-Import
-Core.
-
-Arguments VarPTm {n_PTm}.
-
-Arguments PInd {n_PTm}.
-
-Arguments PSuc {n_PTm}.
-
-Arguments PZero {n_PTm}.
-
-Arguments PNat {n_PTm}.
-
-Arguments PBot {n_PTm}.
-
-Arguments PUniv {n_PTm}.
-
-Arguments PBind {n_PTm}.
-
-Arguments PProj {n_PTm}.
-
-Arguments PPair {n_PTm}.
-
-Arguments PApp {n_PTm}.
-
-Arguments PAbs {n_PTm}.
+Import Core.
 
 #[global]Hint Opaque subst_PTm: rewrite.
 
