theories/common.v
@@ -4,6 +4,7 @@ Import Ltac2.Notations.
 Import Ltac2.Control.
 From Hammer Require Import Tactics.
 
+
 Definition renaming_ok {n m} (Γ : fin n -> PTm n) (Δ : fin m -> PTm m) (ξ : fin m -> fin n) :=
   forall (i : fin m), ren_PTm ξ (Δ i) = Γ (ξ i).
 
